\begin{frame}
  \frametitle{First Returns}
  
  \begin{itemize}
  \item<2->
    $
    N(1,1,2n-2) = \binom{2n-2}{(2n-2)/2} = \binom{2n-2}{n-1} $
  \item<3->
   $ N(-1,1,2n-2) = \binom{2n-2}{(2n-2+2)/2} = \binom{2n-2}{n} $
  \end{itemize}
  
\end{frame}

\begin{frame}
  \frametitle{First Returns}

  \visible<1->{$$N_{\textrm{first\ return}(2n) = N(1,1,2n-2) - N(-1,1,2n-2)$$}
  \visible<2->{$$ = \binom{2n-2}{n-1} - \binom{2n-2}{n} $$}
  \visible<3->{$$ = \frac{(2n-2)!}{(n-1)!(n-1)!} - \frac{(2n-2)!}{n!(n-2)!} $$}
  \visible<4->{$$ = \frac{(2n-2)!}{(n-1)!(n-1)!} - \frac{(2n-2)!}{\alert{(n-1)!(n-1)!}}\alert{\frac{(n-1)}{n}} $$}
  
\end{frame}



\begin{frame}
  \frametitle{First Returns}

  \visible<1->{$$N_{\textrm{first\ return}(2n) = \frac{(2n-2)!}{(n-1)!(n-1)!} - \frac{(2n-2)!}{{(n-1)!(n-1)!}}{\frac{(n-1)}{n}} $$}
  \visible<2->{$$ = \frac{(2n-2)!}{(n-1)!(n-1)!} \left( 1 - \frac{n-1}{n} \right) $$}
  \visible<3->{$$ = \frac{(2n-2)!}{(n-1)!(n-1)!} \left( 1 - 1 + \frac{1}{n} \right) $$}
  \visible<4->{$$ = \frac{1}{n}\frac{(2n-2)!}{(n-1)!(n-1)!} $$}

% ??? Catalan numbers

\end{frame}

\begin{frame}
  \frametitle{First Returns}
  
  \begin{block}{Time for Stirling's Sterling Approximation:}
    $$ \boxed{ n! \simeq \sqrt{2\pi} n^{n+1/2}e^{-n}} $$\cite{abramowitz1974a,gradshteyn1965a}
  \end{block}
  $$( \mbox{good for} \  n \ \mbox{is large}) $$

%  \visible<2->{
%    More generally:
%    $\Gamma(z) \simeq \frac{\sqrt{\pi}}{e} z^{z-1/2}e^{-z}$
%  }

\end{frame}

\begin{frame}[t]
  \frametitle{First Returns}
  \visible<1->{$$N_{\textrm{first\ return}(2n) = \frac{1}{n}\frac{(2n-2)!}{[(n-1)!]^2} $$}
  \visible<2->{$$
    \simeq
    \frac{1}{n}
    \frac{
      \sqrt{2\pi} (2n-2)^{2n-2+1/2} e^{-(2n-2)}
    }
    {
      [\sqrt{2\pi} (n-1)^{n-1+1/2} e^{-(n-1)}]^2
    }
    $$}
  \visible<3->{$$
    =
    \frac{1}{n}
    \frac{
      \sqrt{2\pi} \alert{2^{2n-2+1/2}} (n-1)^{2n-2+1/2} e^{-(2n-2)}
    }
    {
      \alert{\sqrt{2\pi}^2 (n-1)^{2n-2+1} e^{-(2n-2)}}
    }
    $$}%
  \visible<4->{$$
    =
    \frac{1}{n}
    \frac{
      \alert{\cancel{\sqrt{2\pi}}}2^{2n-2+1/2} (n-1)^{2n-2+1/2} e^{-(2n-2)}
    }
    {
      \alert{\sqrt{2\pi}^{\cancel{2}}} (n-1)^{2n-2+1} e^{-(2n-2)}
    }
    $$}%
  \visible<5->{$$
    =
    \frac{1}{n}
    \frac{
      \alert{\cancel{\sqrt{2\pi}}}2^{2n-2+1/2} \alert{\cancel{(n-1)^{2n-2+1/2}}} e^{-(2n-2)}
    }
    {
      \alert{\sqrt{2\pi}^{\cancel{2}}} \alert{\cancel{(n-1)^{2n-2+1/2}}} (n-1)^{1/2} e^{-(2n-2)}
    }
    $$}
\end{frame}

\begin{frame}[t]
  \frametitle{First Returns}
  \visible<1->{$$
    =
    \frac{1}{n}
    \frac{
      \alert{\cancel{\sqrt{2\pi}}}2^{2n-2+1/2} \alert{\cancel{(n-1)^{2n-2+1/2}}} e^{-(2n-2)}
    }
    {
      \alert{\sqrt{2\pi}^{\cancel{2}}} \alert{\cancel{(n-1)^{2n-2+1/2}}} (n-1)^{1/2} e^{-(2n-2)}
    }
    $$}

  \visible<2->{$$
    =
    \frac{1}{n}
    \frac{
      \alert{\cancel{\sqrt{2\pi}}}2^{2n-2+1/2} \alert{\cancel{(n-1)^{2n-2+1/2}}} \alert{\cancel{e^{-(2n-2)}}}
    }
    {
      \alert{\sqrt{2\pi}^{\cancel{2}}} \alert{\cancel{(n-1)^{2n-2+1/2}}} (n-1)^{1/2} \alert{\cancel{e^{-(2n-2)}}}
    }
    $$}
  \visible<3->{$$
    =
    \frac{1}{n}
    \frac{
      2^{2n-3/2} 
    }
    {
      \sqrt{2\pi} (n-1)^{1/2}
    }
    $$}
  \visible<4->{$$
    \sim 
    \alertb{
      \frac{
        2^{2n-3/2}
      }
      {
        \sqrt{2 \pi} n^{3/2}
      }
    }.
    $$}

\end{frame}

\section{Simon's\ model}

\begin{frame}
  \frametitle{Random Competitive Replication}

  \begin{itemize}
  \item <1->
    $$  \frac{n_k}{n_{k-1}}
    =
    \frac{(k-1)(1-\simonalpha)}
    {1+(1-\simonalpha)k}
    $$ 
  \item <2->
    Rearrange:
    $$
    = \frac{k(1-\simonalpha) - (1-\simonalpha)}
    {k(1-\simonalpha) + 1}
    $$
  \item <3->
    Divide through by $k(1-\simonalpha)$:
    $$
    \visible<4->{\frac{1 - \frac{1}{k}}
    {\visible<5->{ 1 + \frac{1}{k(1-\simonalpha)}}}
    }
    $$

  \end{itemize}
  
\end{frame}

\begin{frame}
  \frametitle{Random Competitive Replication}

  \begin{itemize}
  \item  
    $$
    \frac{n_k}{n_{k-1}} =
    \frac{1 - \frac{1}{k}}
    { 1 + \frac{1}{k(1-\simonalpha)}}
    $$
  \item<2-> Use 
    $$ \frac{1}{1+x} = 1 - x + x^2 -x^3 + \ldots $$
  \item<3->
    $$
    \frac{n_k}{n_{k-1}} =
    \left(
      1 - \frac{1}{k}
    \right)
    \left(
      1 - \frac{1}{k(1-\simonalpha)} + O(k^{-2})
    \right)
    $$
  \item<4->
    $$
    =
    1 - \frac{1}{k}
    - \frac{1}{k(1-\simonalpha)} + O(k^{-2})
    $$
  \end{itemize}
\end{frame}


\begin{frame}
  \frametitle{Random Competitive Replication}
  
  \begin{itemize}
  \item<1-> 
    $$ 
    \frac{n_k}{n_{k-1}}
    =
    1 - \frac{1}{k}
    - \frac{1}{k(1-\simonalpha)} + O(k^{-2})
    $$
  \item<1-> 
    $$ 
    \frac{n_k}{n_{k-1}}
    =
    1 
    - \frac{1}{k}
    \left(
      \frac{(1-\simonalpha) + 1}{1-\simonalpha}
    \right)
    + O(k^{-2})
    $$
  \item<2->
    $$
    = 1 - \frac{1}{k}\frac{(2-\simonalpha)}{(1-\simonalpha)}
    + O(k^{-2})
    $$
  \item<3->
    Use
    $$(1+x)^\theta = 1 + \theta x + O(x^2)$$
  \item<4->
    $$
    \frac{n_k}{n_{k-1}}
    = (1 - \frac{1}{k})^{\frac{(2-\simonalpha)}{(1-\simonalpha)}}
    + O(k^{-2})
    $$
  \end{itemize}

\end{frame}
